tinyfstar-new : TyAbs case almost done.
The proof on paper works now with ewf, but F* does not go until the end …

examples/metatheory/tinyfstar-new.fst
@@ -444,8 +444,16 @@ Cmp m (tsubst s t) (tsubst s wp)
 val sub_elam : s:sub -> Tot sub
 let sub_elam s = Sub (esub_elam s) (tsub_elam s)
 
+val esub_elam_at0 : s:sub -> Lemma (Sub.es (sub_elam s) 0 = EVar 0)
+let esub_elam_at0 s = ()
+
 val sub_tlam : s:sub -> Tot sub
 let sub_tlam s = Sub (esub_tlam s) (tsub_tlam s)
+
+let sub_einc = Sub esub_inc tsub_id
+
+
+let sub_tinc s = Sub esub_id (fun x -> TVar (x+1))
 
 val etsubst : s:tsub -> e:exp -> Tot exp
 val ttsubst : s:tsub -> t:typ -> Tot typ
@@ -1169,9 +1177,9 @@ type typing : env -> exp -> cmp -> Type =
 | TyAbs : #g:env ->
           #t1:typ ->
           #ebody:exp ->
-          #m:eff ->
-          #t2:typ ->
-          #wp:typ ->
+          m:eff ->
+          t2:typ ->
+          wp:typ ->
           =hk:kinding g t1 KType ->
            typing (eextend t1 g) ebody (Cmp m t2 wp) ->
            typing g (ELam t1 ebody) (tot (TArr t1 (Cmp m t2 wp)))
@@ -1531,6 +1539,20 @@ let subst_on_econst s ec = ()
 val subst_on_teconst : s:sub -> ec:econst -> Lemma (tsubst s (econsts ec) = econsts ec)
 let subst_on_teconst s ec = admit()
 
+val subst_on_tarrow : s:sub -> t1:typ -> m:eff -> t2:typ -> wp:typ ->
+Lemma (tsubst s (TArr t1 (Cmp m t2 wp)) = TArr (tsubst s t1) (Cmp m (tsubst (sub_elam s) t2) (tsubst (sub_elam s) wp)))
+let subst_on_tarrow s t1 m t2 wp = admit()
+
+val subst_on_elam : s:sub -> t1:typ -> ebody : exp ->
+Lemma (esubst s (ELam t1 ebody) = ELam (tsubst s t1) (esubst (sub_elam s) ebody))
+let subst_on_elam s t1 ebody = admit()
+
+val tsubst_elam_shift : s:sub -> t:typ -> Lemma (tsubst (sub_elam s) (tesh t) = tesh (tsubst s t))
+let tsubst_elam_shift s t = admit()
+
+val ksubst_elam_shift : s:sub -> k:knd -> Lemma (ksubst (sub_elam s) (kesh k) = kesh (ksubst s k))
+let ksubst_elam_shift s k = admit()
+
 val tyif01 : s:sub -> e0:exp -> e1:exp -> e2:exp -> Lemma (esubst s (EIf0 e0 e1 e2) = EIf0 (esubst s e0) (esubst s e1) (esubst s e2))
 let tyif01 s e0 e1 e2 = ()
 val tyif02 : s:sub -> m:eff -> wp0:typ -> Lemma(csubst s (Cmp m tint wp0) = Cmp m tint (tsubst s wp0))
@@ -1599,7 +1621,6 @@ val typing_substitution : #g1:env -> #e:exp -> #c:cmp -> s:sub -> #g2:env ->
     hs:subst_typing s g1 g2 ->
     Tot (typing g2 (esubst s e) (csubst s c))
 *)
-(*
 let rec typing_substitution g1 e c s g2 h1 hs = 
 (*
 | TyVar : #g:env -> x:var{is_Some (lookup_evar g x)} ->
@@ -1620,12 +1641,12 @@ let rec typing_substitution g1 e c s g2 h1 hs =
            typing g (ELam t1 ebody) (tot (TArr t1 (Cmp m t2 wp)))
 *)
 match h1 with 
-(*| TyVar #g1 x hk -> (subst_on_tot s (Cmp.t c); SubstTyping.ef hs x (kinding_substitution s hk hs))*)
-| TyConst g ec h ->
+| TyVar #g1 x hk -> (subst_on_tot s (Cmp.t c); SubstTyping.ef hs x)
+| TyConst g ec hwf ->
     (subst_on_econst s ec;
      subst_on_tot s (econsts ec);
      subst_on_teconst s ec;
-     TyConst g2 ec h)
+     TyConst g2 ec (SubstTyping.hwf2 hs))
 | TyIf0 g e0 e1 e2 m t wp0 wp1 wp2 he0 he1 he2 -> 
 (* Does not work for now …*)
 (
@@ -1649,7 +1670,78 @@ type subst_typing : s:sub -> g1:env -> g2:env -> Type =
                 tf:(a:var{is_Some (lookup_tvar g1 a)} -> Tot(kinding g2 (Sub.ts s a) (ksubst s (Some.v (lookup_tvar g1 a))))) ->
                 subst_typing s g1 g2
 *)
-| TyAbs #g1 #t1 #ebody #m #t2 #wp hk hbody  -> (
+(*
+-----lambda omega version-----
+  | TyLam #gtemp tlam #ebody #tfun hkind hbody ->
+     let hs'' : subst_typing (esub_inc) (g2) (extend_evar g2 0 tlam) =
+       fun x hkind ->
+         TyVar (x+1) (kinding_extensional hkind (extend_evar g2 0 tlam)) in
+     let hs' : subst_typing (esub_lam s) (extend_evar g1 0 tlam)
+                                         (extend_evar g2 0 tlam) =
+       fun y hkindg1 ->
+         if y = 0
+         then TyVar y (kinding_extensional hkindg1 (extend_evar g2 0 tlam))
+         else let hgamma2 = hs (y - 1) (kinding_extensional hkindg1 g1) in
+              substitution esub_inc hgamma2 hs''
+     in (esub_lam_hoist tlam ebody s;
+         TyLam tlam (kinding_extensional hkind g2)
+               (substitution (esub_lam s) hbody hs'))
+-----lambda omega version-----
+*)
+| TyAbs #g1 #t1 #ebody m t2 wp hk hbody  -> 
+(
+let hwfg1ext : ewf (eextend t1 g1) = GType hk in
+let hkt1g2 : kinding g2 (tsubst s t1) KType = kinding_substitution s hk hs in
+let hwfg2ext : ewf (eextend (tsubst s t1) g2) = GType hkt1g2 in
+let hs'' : subst_typing sub_einc g2 (eextend (tsubst s t1) g2) =
+  SubstTyping (SubstTyping.hwf2 hs) hwfg2ext 
+              (fun x -> 
+                         TyVar (x+1) hwfg2ext
+              ) 
+              (fun x -> KVar x hwfg2ext) in
+let hs' : subst_typing (sub_elam s) (eextend t1 g1) (eextend (tsubst s t1) g2) =
+SubstTyping hwfg1ext hwfg2ext 
+(fun x -> match x with 
+	  | 0 -> (*TyVar 0 hwg2ext -> typing g2ext (EVar 0) (tot (shift (tsubst s t1)))
+	          elam_shift       -> typing g2ext (EVar 0) (tot (tsubst (sub_elam s) (sh t1)))*)
+	          (tsubst_elam_shift s t1;
+		   TyVar 0 hwfg2ext)
+          | n -> ( 
+                 (*hg2   -> typing g2 (s.es (x-1)) (tot (tsubst s (g1 (x-1))))*) 
+		 (*ind   -> typing g2ext (shift s.ex (x-1)) (shift (tot (tsubst s (g1 (x-1))))) *)
+		 (*subst_on_tot -> typing g2ext (shift s.ex (x-1)) (tot (shift (tsubst s (g1 (x-1)))))*)
+		 (*elam_shift -> typing g2ext (shift s.ex (x-1)) (tot (tsubst (sub_elam s) (shift (g1 (x-1))))) *)
+		 (* =    -> typing g2ext (esub_elam x) (tot (tsubst (sub_elam s) (g1ext x)))*)
+	         let hg2 = SubstTyping.ef hs (x-1) in
+                 let hg2ext = typing_substitution sub_einc hg2 hs'' in
+		 subst_on_tot sub_einc (tsubst s (Some.v (lookup_evar g1 (x-1))));
+		 tsubst_elam_shift s (Some.v (lookup_evar g1 (x-1)));
+		 hg2ext
+	         )
+)
+(fun a -> let hkg2 = SubstTyping.tf hs a in
+          (*hkg2    -> kinding g2 (s.tf a) (ksubst s (g1 a)) *)
+          let hkg2ext = kinding_substitution sub_einc hkg2 hs'' in
+	  (*hkg2ext -> kinding g2ext (tesh (s.tf a)) (kesh (ksubst s (g1 a)))*)
+	  (*elam_shift -> kinding g2ext (tesh (s.tf a)) (ksubst (sub_elam s) (kesh (g1 a)))*)
+	  ksubst_elam_shift s (Some.v (lookup_tvar g1 a));
+	  hkg2ext
+)
+in
+let hbodyg2ext : typing (eextend (tsubst s t1) g2) (esubst (sub_elam s) ebody) (Cmp m (tsubst (sub_elam s) t2) (tsubst (sub_elam s) wp)) = typing_substitution (sub_elam s) hbody hs' in
+(*hbodyg2ext -> typing (eextend (tsubst s t1) g2) (esubst (sub_elam s) ebody) (Cmp m (tsubst s t2) (tsubst s wp)) *)
+let habsg2ext = TyAbs m (tsubst (sub_elam s) t2) (tsubst (sub_elam s) wp) hkt1g2 hbodyg2ext in
+(*habsg2ext  -> typing g2 (ELam (tsubst s t1) (esubst (sub_elam s) ebody)) (tot (TArr (tsubst s t1) (Cmp m (tsubst (sub_elam s) t2) (tsubst (sub_elam s) wp))))*)
+subst_on_elam s t1 ebody;
+let habsg2ext' : typing g2 (esubst s (ELam t1 ebody)) (tot (TArr (tsubst s t1) (Cmp m (tsubst (sub_elam s) t2) (tsubst (sub_elam s) wp)))) = habsg2ext in
+subst_on_tarrow s t1 m t2 wp;
+let habsg2ext'' : typing g2 (esubst s (ELam t1 ebody)) (tot (tsubst s (TArr t1 (Cmp m t2 wp)))) = habsg2ext' in
+subst_on_tot s (TArr t1 (Cmp m t2 wp));
+assert (tot (tsubst s (TArr t1 (Cmp m t2 wp))) = csubst s (tot (TArr t1 (Cmp m t2 wp))));
+(*
+let habsg2extppp : typing g2 (esubst s (ELam t1 ebody)) (csubst s (tot (TArr t1 (Cmp m t2 wp)))) = habsg2ext'' in
+*)
+admit()
 (*let hs'' : subst_typing sub_inc g2 (eextend g2 0 t1) = admit() in
 let hs' : subst_typing (sub_elam s) (eextend t1 g1) (eextend (tsubst s t1) g2) = admit()
 (*
@@ -1661,7 +1753,6 @@ match x with
 | _ -> let hgamma2 =  
 *)
 in*)
-admit()
 )
 | _ -> admit()
 and scmp_substitution g1 c1 c2 phi s g2 h1 hs = admit()
@@ -1827,5 +1918,4 @@ val v_eq_symt : #g:env -> #t1:typ -> #t2:typ -> #k:knd ->
             =hv:validity g (teqt k t1 t2) ->
                 validity g (teqt k t2 t1)
 let v_eq_symt = admit()
-*)
 *)
